Add core candidate execution definitions

ArchSem/CandidateExecution.lean
@@ -2,10 +2,565 @@
 --
 -- SPDX-License-Identifier: Apache-2.0 OR BSD-2-Clause
 
-import Std.Data.HashSet
+import Std.Data.ExtTreeSet
+import ArchSem.Trace
+import Sail.ArchSem
+import ArchSem.Defs
+import ArchSem.TerminatingModel
+
+open Sail.ArchSem
+open ArchSem.TerminatingModel
+
+-- TODO: add comments
 
 namespace ArchSem.CandidateExecutions
 
-abbrev Rel (α : Type) [Hashable α] [BEq α] := Std.HashSet (α × α)
+abbrev Rel (α : Type) (cmp : α × α → α × α → Ordering := by exact compare) := Std.ExtTreeSet (α × α) cmp
+
+namespace Rel
+
+def union {α : Type} {cmp : α × α → α × α → Ordering} [Std.TransCmp cmp]
+    (r₁ r₂ : Rel α cmp) : Rel α cmp :=
+  Std.ExtTreeSet.union r₁ r₂
+
+def intersection {α : Type} {cmp : α × α → α × α → Ordering} [Std.TransCmp cmp]
+    (r₁ r₂ : Rel α cmp) : Rel α cmp :=
+  Std.ExtTreeSet.inter r₁ r₂
+
+end Rel
+
+
+abbrev IMon [Arch] := FreeM (InstructionEffect ⊕ FinChoice)
+def IEvent [Arch] : Type := FreeM.Event InstructionEffect
+def ITrace [Arch] : Type → Type := FreeM.Trace InstructionEffect
+
+namespace IEvent
+
+variable [Arch]
+
+def getReg (ev : IEvent) : Option Arch.register :=
+  match ev.call with
+  | .regRead reg _ => .some reg
+  | .regWrite reg _ _ => .some reg
+  | _ => .none
+
+
+def getRegValue (ev : IEvent)
+    : Option (Σ (r : Arch.register), Arch.register_type r) :=
+  match h : ev.call with
+  | .regRead reg _ =>
+    have h_eq : Arch.register_type reg = InstructionEffect.ret ev.call := by
+      simp [InstructionEffect.ret, h]
+    let val : Arch.register_type reg := h_eq ▸ ev.ret
+    .some ⟨reg, val⟩
+  | .regWrite reg _ val => .some ⟨reg, val⟩
+  | _ => .none
+
+def getMemRequest (ev : IEvent) : Option MemRequest :=
+  match ev.call with
+  | .memRead memReq => .some memReq
+  | .memWriteAnnounce memReq => .some memReq
+  | .memWrite memReq _ _ => .some memReq
+  | _ => .none
+
+def getAddr (ev : IEvent) : Option Address := do
+  let memReq ← ev.getMemRequest
+  return memReq.address
+
+def getMemValue (ev : IEvent) : Option (Σ n : Nat, BitVec (8 * n)) :=
+  match h : ev.call with
+  | .memRead req =>
+    have h_eq : Except Arch.abort (BitVec (8 * req.size) × BitVec req.numTag) = Effect.ret ev.call := by
+      simp [Effect.ret, InstructionEffect.ret, h]
+    match (h_eq ▸ ev.ret) with
+    | Except.ok (val, _) => .some ⟨req.size, val⟩
+    | Except.error _ => .none
+  | .memWrite req val _ => .some ⟨req.size, val⟩
+  | _ => .none
+
+def getBarrier (ev : IEvent) : Option Arch.barrier :=
+  match ev.call with
+  | .barrier barrier => .some barrier
+  | _ => .none
+
+def getCacheOp (ev : IEvent) : Option Arch.cache_op :=
+  match ev.call with
+  | .cacheOp op => .some op
+  | _ => .none
+
+def getTlbi (ev : IEvent) : Option Arch.tlbi :=
+  match ev.call with
+  | .tlbOp tlbi => .some tlbi
+  | _ => .none
+
+def getTransStart (ev : IEvent) : Option Arch.trans_start :=
+  match ev.call with
+  | .translationStart ts => .some ts
+  | _ => .none
+
+def getTransEnd (ev : IEvent) : Option Arch.trans_end :=
+  match ev.call with
+  | .translationEnd te => .some te
+  | _ => .none
+
+section IsReg
+
+variable (ev : IEvent) (p : (r : Arch.register) → Option Arch.sys_reg_id → Arch.register_type r → Prop)
+
+def is_reg_read_with : Prop
+  := match h : ev.call with
+  | .regRead reg racc =>
+    have h_eq : Arch.register_type reg = InstructionEffect.ret ev.call := by
+      simp [InstructionEffect.ret, h]
+    let val : Arch.register_type reg := h_eq ▸ ev.ret
+    p reg racc val
+  | _ => False
+
+instance [h : ∀ r acc v, Decidable (p r acc v)] : Decidable (is_reg_read_with ev p) := by
+  rw [is_reg_read_with] ; split
+  · apply h
+  · exact Decidable.isFalse False.elim
+
+def is_reg_write_with : Prop
+  := match ev.call with
+  | .regWrite reg racc val => p reg racc val
+  | _ => False
+
+instance [h : ∀ r acc v, Decidable (p r acc v)] : Decidable (is_reg_write_with ev p) := by
+  rw [is_reg_write_with] ; split
+  · apply h
+  · exact Decidable.isFalse False.elim
+
+def is_reg_event_with : Prop := is_reg_read_with ev p ∨ is_reg_write_with ev p
+
+end IsReg
+
+def is_mem_read_req_with (ev : IEvent)
+    (p : (req : MemRequest) → Except Arch.abort (BitVec (8 * req.size) × BitVec (req.numTag)) → Prop)
+  := match h : ev.call with
+  | .memRead req =>
+    let h_eq : Except Arch.abort (BitVec (8 * req.size) × BitVec req.numTag) = Effect.ret ev.call := by
+      simp [Effect.ret, InstructionEffect.ret, h]
+    p req (h_eq ▸ ev.ret)
+  | _ => False
+
+instance [h : ∀ req res, Decidable (p req res)] : Decidable (is_mem_read_req_with ev p) := by
+  rw [is_mem_read_req_with] ; split
+  · apply h
+  · exact Decidable.isFalse False.elim
+
+def is_mem_read_with (ev : IEvent)
+    (p : (req : MemRequest) → BitVec (8 * req.size) → BitVec req.numTag → Prop) : Prop
+  := is_mem_read_req_with ev (fun req res => match res with
+       | .ok val => p req val.fst val.snd
+       | .error _ => False)
+
+instance [h : ∀ req val tags, Decidable (p req val tags)]
+    : Decidable (is_mem_read_with ev p) := by
+  rw [is_mem_read_with, is_mem_read_req_with] ; split
+  · split
+    · apply h
+    · exact Decidable.isFalse False.elim
+  · exact Decidable.isFalse False.elim
+
+def is_mem_write_announce_with (ev : IEvent) (p : MemRequest → Prop) :=
+  match ev.call with
+  | .memWriteAnnounce req => p req
+  | _ => False
+
+instance [h : ∀ req, Decidable (p req)] : Decidable (is_mem_write_announce_with ev p) := by
+  rw [is_mem_write_announce_with] ; split
+  · apply h
+  · exact Decidable.isFalse False.elim
+
+def is_mem_write_req_with (ev : IEvent)
+    (p : (req : MemRequest) → BitVec (8 * req.size) → BitVec req.numTag → Except Arch.abort Unit → Prop) : Prop
+  := match h : ev.call with
+  | .memWrite req val tags =>
+    let h_eq : Except Arch.abort Unit = Effect.ret ev.call := by
+      simp [Effect.ret, InstructionEffect.ret, h]
+    p req val tags (h_eq ▸ ev.ret)
+  | _ => False
+
+instance [h : ∀ req val tags res, Decidable (p req val tags res)]
+    : Decidable (is_mem_write_req_with ev p) := by
+  rw [is_mem_write_req_with] ; split
+  · apply h
+  · exact Decidable.isFalse False.elim
+
+def is_mem_write_with (ev : IEvent)
+    (p : (req : MemRequest) → BitVec (8 * req.size) → BitVec req.numTag → Prop) : Prop
+  := is_mem_write_req_with ev (fun req val tags res => match res with
+       | .ok () => p req val tags
+       | .error _ => False)
+
+instance [h : ∀ req val tags, Decidable (p req val tags)]
+    : Decidable (is_mem_write_with ev p) := by
+  rw [is_mem_write_with, is_mem_write_req_with] ; split
+  · split
+    · apply h
+    · exact Decidable.isFalse False.elim
+  · exact Decidable.isFalse False.elim
+
+def is_barrier_with (ev : IEvent) (p : Arch.barrier → Prop) : Prop
+  := match ev.call with
+  | .barrier barrier => p barrier
+  | _ => False
+
+instance [h : ∀ barrier, Decidable (p barrier)]
+    : Decidable (is_barrier_with ev p) := by
+  rw [is_barrier_with] ; split
+  · apply h
+  · exact Decidable.isFalse False.elim
+
+def is_cache_op_with (ev : IEvent) (p : Arch.cache_op → Prop) : Prop
+  := match ev.call with
+  | .cacheOp op => p op
+  | _ => False
+
+instance [h : ∀ op, Decidable (p op)]
+    : Decidable (is_cache_op_with ev p) := by
+  rw [is_cache_op_with] ; split
+  · apply h
+  · exact Decidable.isFalse False.elim
+
+def is_tlb_op_with (ev : IEvent) (p : Arch.tlbi → Prop) : Prop
+  := match ev.call with
+  | .tlbOp op => p op
+  | _ => False
+
+instance [h : ∀ op, Decidable (p op)]
+    : Decidable (is_tlb_op_with ev p) := by
+  rw [is_tlb_op_with] ; split
+  · apply h
+  · exact Decidable.isFalse False.elim
+
+abbrev is_reg_read (ev : IEvent) := is_reg_read_with ev (fun _ _ _ => True)
+abbrev is_reg_write (ev : IEvent) := is_reg_write_with ev (fun _ _ _ => True)
+abbrev is_reg_event (ev : IEvent) := is_reg_event_with ev (fun _ _ _ => True)
+abbrev is_mem_read_req (ev : IEvent) := is_mem_read_req_with ev (fun _ _ => True)
+abbrev is_mem_read (ev : IEvent) := is_mem_read_with ev (fun _ _ _ => True)
+abbrev is_mem_write_announce (ev : IEvent) := is_mem_write_announce_with ev (fun _ => True)
+abbrev is_mem_write_req (ev : IEvent) := is_mem_write_req_with ev (fun _ _ _ _ => True)
+abbrev is_mem_write (ev : IEvent) := is_mem_write_with ev (fun _ _ _ => True)
+abbrev is_barrier (ev : IEvent) := is_barrier_with ev (fun _ => True)
+abbrev is_cache_op (ev : IEvent) := is_cache_op_with ev (fun _ => True)
+abbrev is_tlb_op (ev : IEvent) := is_tlb_op_with ev (fun _ => True)
+
+def is_unsupported_event (ev : IEvent) : Prop :=
+  is_mem_read_req_with ev (fun req _ => req.numTag ≠ 0) ∨
+  is_mem_write_req_with ev (fun req _ _ _ => req.numTag ≠ 0)
+
+end IEvent
+
+inductive ITrace.matches_isa [Arch]
+    : IMon α → ITrace α → Prop
+  | stopped (f : FreeM (InstructionEffect ⊕ FinChoice) α) : matches_isa f .stopped
+  | ret (a : α) : matches_isa (.pure a) (.ret a)
+  | eff (eff : InstructionEffect) (k : eff.ret → FreeM (InstructionEffect ⊕ FinChoice) α)
+      : matches_isa (.impure (.inl eff) k) (.openCall eff)
+  | next (eff : InstructionEffect) (k : eff.ret → IMon α) (ret : eff.ret)
+      (t : ITrace α)
+      : matches_isa (k ret) t → matches_isa (.impure (.inl eff) k) (.cons (eff &→ ret) t)
+  | choose (n : Nat) (i : Fin n) (k : Fin n → IMon α) (t : ITrace α)
+      : matches_isa (k i) t → matches_isa (.impure (.inr n) k) t
+
+structure Eid where
+  tid : Nat
+  iid : Nat
+  ieid : Nat
+deriving BEq
+
+-- TODO: other Eid ordering relations?
+
+def Eid.compare (a b : Eid) : Ordering :=
+  if a.tid < b.tid
+  then .lt
+  else if a.tid > b.tid
+  then .gt
+  else if a.iid < b.iid
+  then .lt
+  else if a.iid > b.iid
+  then .gt
+  else if a.ieid < b.ieid
+  then .lt
+  else if a.ieid > b.ieid
+  then .gt
+  else .eq
+
+instance : Ord Eid where
+  compare := Eid.compare
+
+instance : Std.TransCmp Eid.compare where
+  isLE_trans := by sorry
+  eq_swap := by sorry
+
+instance : Std.TransCmp (compare : Eid → Eid → Ordering) := by
+  change Std.TransCmp Eid.compare
+  infer_instance
+
+-- TODO: Eid ordering relations
+
+structure PreCand [Arch] [ArchExtra] (nThreads : Nat) where
+  init : ArchState nThreads
+  events : Vector (List (ITrace Unit)) nThreads
+
+namespace PreCand
+
+variable [Arch] [ArchExtra]
+
+def matches_isa (p : PreCand nThreads) (isem : IMon Unit) : Prop :=
+  ∀ (tid : Fin nThreads), ∀ trace ∈ p.events[tid], trace.matches_isa isem
+
+def is_complete (p : PreCand nThreads) : Prop :=
+  ∀ (tid : Fin nThreads), ∀ trace ∈ p.events[tid], trace.snd = .ret ()
+
+def lookupInstruction (p : PreCand nThreads) (tid iid : Nat)
+    : Option (ITrace Unit) := do
+  let threadTraces ← p.events[tid]?
+  threadTraces[iid]?
+
+def instructionList (p : PreCand nThreads) : List (Nat × Nat × ITrace Unit) :=
+  p.events.toList.mapIdx
+    (fun tid traces => traces.mapIdx (fun iid trace => (tid, iid, trace)))
+  |>.flatten
+
+theorem lookup_instruction_list (p : PreCand nThreads) (tid iid : Nat) (t : ITrace Unit)
+    : lookupInstruction p tid iid = .some t ↔ (tid, iid, t) ∈ instructionList p := by
+  sorry
+
+def lookupIEvent (p : PreCand nThreads) (tid iid ieid : Nat) : Option IEvent := do
+  let inst ← p.lookupInstruction tid iid
+  inst.fst[ieid]?
+
+def iEventList (p : PreCand nThreads) : List (Nat × Nat × Nat × IEvent) :=
+  p.instructionList.map
+    (fun (tid, iid, trace) => trace.fst.mapIdx (fun ieid ev => (tid, iid, ieid, ev)))
+  |>.flatten
+
+theorem lookup_ievent_list (p : PreCand nThreads) (tid iid ieid : Nat) (ev : IEvent)
+    : lookupIEvent p tid iid ieid = .some ev ↔ (tid, iid, ieid, ev) ∈ p.iEventList := by
+  sorry
+
+def iEventList' (p : PreCand nThreads) : List (Eid × IEvent) :=
+  p.iEventList |>.map (fun (tid, iid, ieid, ev) => ({tid, iid, ieid}, ev))
+
+def eid_valid (p : PreCand nThreads) (eid : Eid) : Prop :=
+  (lookupIEvent p eid.tid eid.iid eid.ieid).isSome
+
+instance (p : PreCand nThreads) (eid : Eid) : Decidable (eid_valid p eid) := by
+  simp [eid_valid]
+  infer_instance
+
+instance : GetElem (PreCand nThreads) Eid IEvent eid_valid where
+   getElem (p : PreCand nThreads) (eid : Eid) (h : eid_valid p eid) : IEvent := by
+     match h_lookup : lookupIEvent p eid.tid eid.iid eid.ieid with
+     | .some ev => exact ev
+     | .none =>
+       rw [eid_valid] at h
+       rw [←Option.not_isSome_iff_eq_none] at h_lookup
+       contradiction
+
+def collectEid (f : Eid → IEvent → Prop) (p : PreCand nThreads)
+    [h : ∀ eid ev, Decidable (f eid ev)]
+    : Std.ExtTreeSet Eid :=
+  Std.ExtTreeSet.ofList (
+    p.iEventList'
+    |>.filter (fun (eid, event) => f eid event)
+    |>.map Prod.fst
+  )
+
+def eids (p : PreCand nThreads) : Std.ExtTreeSet Eid := p.collectEid (fun _ _ => True)
+
+def regReads (p : PreCand nThreads) : Std.ExtTreeSet Eid :=
+  p.collectEid (fun _ ev => IEvent.is_reg_read ev)
+def pcReads (p : PreCand nThreads) : Std.ExtTreeSet Eid :=
+  p.collectEid (fun _ ev => IEvent.is_reg_read_with ev (fun reg _ _ => reg = ArchExtra.register_pc))
+
+def regWrites (p : PreCand nThreads) : Std.ExtTreeSet Eid :=
+  p.collectEid (fun _ ev => IEvent.is_reg_write ev)
+def pcWrites (p : PreCand nThreads) : Std.ExtTreeSet Eid :=
+  p.collectEid (fun _ ev => IEvent.is_reg_write_with ev (fun reg _ _ => reg = ArchExtra.register_pc))
+
+def memReads (p : PreCand nThreads) : Std.ExtTreeSet Eid :=
+  p.collectEid (fun _ ev => IEvent.is_mem_read ev)
+def memReadReqs (p : PreCand nThreads) : Std.ExtTreeSet Eid :=
+  p.collectEid (fun _ ev => IEvent.is_mem_read_req ev)
+
+def memReadAborts (p : PreCand nThreads) : Std.ExtTreeSet Eid :=
+  p.collectEid (fun _ ev => IEvent.is_mem_read_req_with ev (fun _ res => not res.isOk))
+
+def memWriteAddrAnnounces (p : PreCand nThreads) : Std.ExtTreeSet Eid :=
+  p.collectEid (fun _ ev => IEvent.is_mem_write_announce ev)
+def memWrites (p : PreCand nThreads) : Std.ExtTreeSet Eid :=
+  p.collectEid (fun _ ev => IEvent.is_mem_write ev)
+def memWriteReqs (p : PreCand nThreads) : Std.ExtTreeSet Eid :=
+  p.collectEid (fun _ ev => IEvent.is_mem_write_req ev)
+def memWriteAborts (p : PreCand nThreads) : Std.ExtTreeSet Eid :=
+  p.collectEid (fun _ ev => IEvent.is_mem_write_req_with ev (fun _ _ _ res => not res.isOk))
+
+def readsByKind (p : PreCand nThreads) (q : Arch.mem_acc → Bool)
+    : Std.ExtTreeSet Eid :=
+  p.collectEid (fun _ ev => IEvent.is_mem_read_with ev (fun req _ _ => q req.accessKind))
+def writesByKind (p : PreCand nThreads) (q : Arch.mem_acc → Bool)
+    : Std.ExtTreeSet Eid :=
+  p.collectEid (fun _ ev => IEvent.is_mem_write_with ev (fun req _ _ => q req.accessKind))
+
+def barriers (p : PreCand nThreads) : Std.ExtTreeSet Eid :=
+  p.collectEid (fun _ ev => IEvent.is_barrier ev)
+def cacheOps (p : PreCand nThreads) : Std.ExtTreeSet Eid :=
+  p.collectEid (fun _ ev => IEvent.is_cache_op ev)
+def tlbOps (p : PreCand nThreads) : Std.ExtTreeSet Eid :=
+  p.collectEid (fun _ ev => IEvent.is_tlb_op ev)
+
+def finalThreadRegisterMap (p : PreCand nThreads) (tid : Fin nThreads) : RegisterMap :=
+  p.events[tid].foldl (fun regMap iTrace =>
+    iTrace.fst.foldl (fun regMap event =>
+      match event.call with
+      | .regWrite reg _acc val =>
+        -- TODO (think about): the operational models are able to throw an error
+        -- here when there is an invalid access type.
+        regMap.insert reg val
+      | _ => regMap
+    ) regMap
+  )
+  p.init.regs[tid]
+
+def finalRegisterMaps (p : PreCand nThreads) : Vector RegisterMap nThreads :=
+  Vector.ofFn (finalThreadRegisterMap p)
+
+-- TODO:
+-- gatherByKey (create map of keys to events)
+-- sameKey (create equivalence relation)
+-- sameThread (equivalence relation)
+-- sameInstructionInstance (equiv rel)
+-- ...
+
+def collectEidByKey {K : Type} [Ord K] [Std.TransCmp (compare : K → K → Ordering)]
+    (p : PreCand nThreads) (getKey : Eid → IEvent → Option K)
+    : Std.ExtTreeMap K (Std.ExtTreeSet Eid) :=
+  p.iEventList'.foldl (fun map (eid, event) =>
+      match getKey eid event with
+      | .some key => map.insert key ((map.getD key (Std.ExtTreeSet.empty (cmp := Eid.compare))).insert eid)
+      | .none => map
+    ) Std.ExtTreeMap.empty
+
+-- TODO: move this function elsewhere
+def setProd {cmp : α → α → Ordering} [Std.TransCmp cmp]
+    {cmp' : α × α → α × α → Ordering} [Std.TransCmp cmp']
+    (a b : Std.ExtTreeSet α cmp) : Std.ExtTreeSet (α × α) cmp' :=
+  a.foldl (fun prod a =>
+    b.foldl (fun prod b =>
+      prod.insert (a, b)
+    ) prod
+  ) Std.ExtTreeSet.empty
+
+def sameKey {K : Type} [Ord K] [Std.TransCmp (compare : K → K → Ordering)]
+    (p : PreCand nThreads) (getKey : Eid → IEvent → Option K)
+    : Rel Eid :=
+  (collectEidByKey p getKey).foldl (fun acc _ eids =>
+    Std.ExtTreeSet.union acc (setProd eids eids)
+  ) Std.ExtTreeSet.empty
+
+def sameThread (p : PreCand nThreads) : Rel Eid :=
+  p.sameKey (fun eid _ => .some eid.tid)
+
+def sameInstructionInstance (p : PreCand nThreads) : Rel Eid :=
+  p.sameKey (fun eid _ => .some (eid.tid, eid.iid))
+
+def intraInstructionOrder (p : PreCand nThreads) : Rel Eid :=
+  p.sameInstructionInstance
+  |>.filter (fun (a,b) => a.ieid < b.ieid)
+
+def interInstructionOrder (p : PreCand nThreads) : Rel Eid :=
+  p.sameThread
+  |>.filter (fun (a,b) => a.iid < b.iid)
+
+def programOrder (p : PreCand nThreads) : Rel Eid :=
+  Rel.union p.interInstructionOrder p.intraInstructionOrder
+
+def sameAddr (p : PreCand nThreads) : Rel Eid :=
+  p.sameKey (fun _ ev => ev.getAddr)
+
+def sameMemValue (p : PreCand nThreads) : Rel Eid :=
+  p.sameKey (fun _ ev => ev.getMemValue)
+
+def sameReg (p : PreCand nThreads) : Rel Eid :=
+  p.sameKey (fun eid ev => Option.map (eid.tid, ·) ev.getReg)
+
+def sameRegSameValue (p : PreCand nThreads) : Rel Eid :=
+  p.sameKey (fun eid ev => Option.map (eid.tid, ·) ev.getRegValue)
+
+-- TODO: finish adding other relations starting from is_valid_init_reg_read and co.
+
+end PreCand
+
+structure Cand (nThreads : Nat) [Arch] [ArchExtra] where
+  pre : PreCand nThreads
+  memReadsFrom : Rel Eid
+  regReadsFrom : Rel Eid
+  coherence : Rel Eid
+  exclusives : Rel Eid
+
+
+namespace Cand
+
+variable [Arch] [ArchExtra]
+
+def eid_valid (c : Cand nThreads) : Eid → Prop := c.pre.eid_valid
+
+instance (c : Cand nThreads) (eid : Eid) : Decidable (eid_valid c eid) := by
+  simp [eid_valid]
+  infer_instance
+
+instance : GetElem (Cand nThreads) Eid IEvent eid_valid where
+  getElem (c : Cand nThreads) (eid : Eid) (valid : c.eid_valid eid) : IEvent
+    := c.pre[eid]
+
+def finalWrites (c : Cand nThreads) : Std.ExtTreeMap Address (Eid × BitVec 8) :=
+  c.pre.iEventList'.foldl (fun mem (eid, ev) =>
+    match ev.call with
+    | .memWrite req val tags =>
+      (List.finRange req.size).foldl (fun mem (i : Fin req.size) =>
+        -- CR clang for thibaut: What happens if this addition overflows?
+        let addr := req.address + i.val
+        let byte := (Sail.bitvec_to_vecbytes val)[i]
+        match mem.get? addr with
+        | .some (eid', byte') =>
+          if c.coherence.contains (eid, eid')
+          then mem.insert addr (eid, byte)
+          else mem
+        | .none => mem.insert addr (eid, byte)
+      ) mem
+    | _ => mem
+  ) Std.ExtTreeMap.empty
+
+def finalMemMap (c : Cand nThreads) : MemoryMap :=
+  let writtenMem := (finalWrites c).map (fun _ (_,v) => v)
+  Std.ExtTreeMap.union c.pre.init.memory writtenMem
+
+def toArchState (c : Cand nThreads) : ArchState nThreads :=
+  { memory := c.finalMemMap
+  , addressSpace := c.pre.init.addressSpace
+  , regs := c.pre.finalRegisterMaps
+  }
+
+def valid_rf (c : Cand nThreads) (wsrc rdst : Eid) : Prop :=
+  Option.isSome (do
+    let write ← c[wsrc]?
+    -- TODO complete this and other similar definitions.
+    return Option.some ()
+  )
+
+end Cand
+
+inductive AxiomaticModel.Behavior (Flag : Type) where
+  | allowed
+  | rejected
+  | flagged (f : Flag)
+
+def AxiomaticModel [Arch] [ArchExtra] (Flag : Type)
+  := (nThreads : Nat) → Cand nThreads
+  → Except String (AxiomaticModel.Behavior Flag)
 
 end ArchSem.CandidateExecutions
